Examples/EdmondsKarp_Maxflow/Augmenting_Path_BFS_Impl.thy
@@ -1,7 +1,8 @@
 theory Augmenting_Path_BFS_Impl
   imports
-          "../../Refine_Imperative_HOL/IICF/Impl/IICF_Rbt_Set"
-          "../../Refine_Imperative_HOL/IICF/Impl/IICF_RbtMap_Map"
+          "../../Refine_Imperative_HOL/IICF/Impl/IICF_List_Set"
+      (*    "../../Refine_Imperative_HOL/IICF/Impl/IICF_RbtMap_Map" *)
+          "../../Refine_Imperative_HOL/IICF/Impl/IICF_ArrayMap_Map"
           Augmenting_Path_BFS 
 begin
 
@@ -30,14 +31,15 @@ term Augmenting_Path_BFS.bfs2
                
 context Impl_Succ begin
 
-    abbreviation "init_state_time == 3 + rbt_insert_logN 1 + rbt_insert_logN 1"
+    abbreviation "init_state_time == 11 + N + rbt_insert_logN 1"
 
 
-    definition "set_pick_time = (10::nat)"
+    definition "set_delete_time vcf = rbt_delete_time_logN (vcf + 1)"
+    definition "set_pick_time vcf = (4::nat)+ (set_delete_time vcf)"
 
-    lemma [simp]: "set_pick_time > (0::nat)" unfolding set_pick_time_def by auto
+    lemma [simp]: "set_pick_time cf > (0::nat)" unfolding set_pick_time_def by auto
 
-definition "map_lookup_time vcf = rbt_search_time_logN (1 +  vcf) + 1" 
+definition "map_lookup_time vcf = (2::nat) " 
 lemma [simp]: "map_lookup_time cf > 0" unfolding map_lookup_time_def by simp
  
  
@@ -45,9 +47,9 @@ lemma [simp]: "map_lookup_time cf > 0" unfolding map_lookup_time_def by simp
 
 
 definition init_state :: "nat \<Rightarrow> (bool \<times> (nat \<Rightarrow> nat option) \<times> nat set \<times> nat set \<times> nat) nrest" where
-  "init_state src = do {
-        m \<leftarrow> mop_map_empty (1::nat);
-        m \<leftarrow> mop_map_update (\<lambda>M. rbt_insert_logN (sizeM1' M)) m src src;
+  "init_state  src  = do {
+        m \<leftarrow> mop_map_empty (N+3);
+        m \<leftarrow> mop_map_update (\<lambda>M. 6) m src src;
         C \<leftarrow> mop_set_empty (1::nat);
         C \<leftarrow> mop_set_insert (\<lambda>_. rbt_insert_logN (card C + 1)) src C;
         N \<leftarrow> mop_set_empty (1::nat);
@@ -56,20 +58,19 @@ definition init_state :: "nat \<Rightarrow> (bool \<times> (nat \<Rightarrow> na
     
     term mop_set_insert
     definition "set_insert_time vcf = rbt_insert_logN (vcf + 1)"
-    definition "set_delete_time vcf = rbt_delete_time_logN (vcf + 1)"
-    definition "map_dom_member_time vcf = rbt_search_time_logN (1 + vcf) + 1"
-    definition "map_update_time vcf = rbt_insert_logN (1 + vcf)" 
+    definition "map_dom_member_time vcf = (2::nat)"
+    definition "map_update_time vcf = (6::nat)" 
     definition "set_isempty_time = (10::nat)"
     definition "set_empty_time = (10::nat)"
     definition "list_append_time = (1::nat)"
 
     abbreviation "bfs2 cf SS IS s t == Augmenting_Path_BFS.bfs2 cf
-                       (set_insert_time (card (Graph.V cf))) (map_dom_member_time (card (Graph.V cf)))  (set_delete_time (card (Graph.V cf))) (map_update_time (card (Graph.V cf)))
-                      set_pick_time list_append_time (map_lookup_time (card (Graph.V cf))) set_empty_time set_isempty_time SS IS s t"
+                       (set_insert_time (card (Graph.V cf))) (map_dom_member_time (card (Graph.V cf))) (map_update_time (card (Graph.V cf)))
+                      (set_pick_time (card (Graph.V cf))) list_append_time (map_lookup_time (card (Graph.V cf))) set_empty_time set_isempty_time SS IS s t"
 
 
     definition op_bfs :: "'ga \<Rightarrow> node \<Rightarrow> node \<Rightarrow> path option nrest"
-      where [simp]: "op_bfs c s t \<equiv> bfs2 (absG c) (succ c) init_state s t"
+      where [simp]: "op_bfs c s t \<equiv> bfs2 (absG c) (succ c) (init_state) s t"
   
    (* lemma pat_op_dfs[pat_rules]: 
       "bfs2$(absG$c)$(succ$c)$s$t \<equiv> UNPROTECT op_bfs$c$s$t" by simp 
@@ -82,34 +83,52 @@ definition init_state :: "nat \<Rightarrow> (bool \<times> (nat \<Rightarrow> na
       = "bool \<times> (node \<rightharpoonup> node) \<times> node set \<times> node set \<times> nat"
  
 
-
-    lemma P: "Pre_BFS_Impl set_pick_time" unfolding Pre_BFS_Impl_def by simp
+ 
  
 
   
   
-  lemma init_state_correct: "init_state src \<le> SPECT [ (False,[src\<mapsto>src],{src},{},0::nat) \<mapsto> init_state_time ]"
+  lemma init_state_correct: "init_state src \<le> SPECT [ (False,[src\<mapsto>src],{src},{},0::nat) \<mapsto> init_state_time  ]"
     unfolding init_state_def   
     apply(rule T_specifies_I) unfolding mop_map_empty_def mop_map_update_def mop_set_empty_def
         mop_set_insert_def
-    by(vcg' \<open>clarsimp\<close>  ) 
+    by(vcg' \<open>clarsimp\<close>  )  
 
 
 
 
-    sepref_register init_state :: "node \<Rightarrow> ibfs_state nrest"
 
     schematic_goal init_state_impl:
       fixes src :: nat
+      assumes src_inbounds: "src < N" 
       notes [id_rules] = 
-        itypeI[Pure.of src "TYPE(nat)"]
+        itypeI[Pure.of src "TYPE(nat)"] 
       shows "hn_refine (hn_val nat_rel src srci) 
-        (?c::?'c Heap) ?\<Gamma>' ?R (init_state src)"
-      using [[id_debug, goals_limit = 1]]
-      unfolding init_state_def   
-      apply sepref 
+        (?c::?'c Heap) ?\<Gamma>' ?R (PR_CONST (init_state) src)"
+      using [[id_debug, goals_limit = 3]]
+      unfolding init_state_def PR_CONST_def   using src_inbounds
+      unfolding mop_map_empty_add_mn[where s="N"] (*
+  apply sepref_dbg_preproc 
+  apply sepref_dbg_cons_init
+  apply sepref_dbg_id 
+     apply sepref_dbg_monadify
+
+     apply sepref_dbg_opt_init
+                                        
+  apply sepref_dbg_trans_keep
+
+  apply sepref_dbg_opt
+  apply sepref_dbg_cons_solve \<comment> \<open>Frame rule, recovering the invalidated list 
+    or pure elements, propagating recovery over the list structure\<close>
+  apply sepref_dbg_cons_solve \<comment> \<open>Trivial frame rule\<close>
+  apply sepref_dbg_constraints *)
+      apply sepref
       done
-      concrete_definition (in -) init_state_impl uses Impl_Succ.init_state_impl
+concrete_definition (in -) init_state_impl uses Impl_Succ.init_state_impl
+    print_theorems
+
+    sepref_register "init_state " :: " node \<Rightarrow> ibfs_state nrest"
+
 
       thm init_state_impl_def
 
@@ -118,7 +137,7 @@ definition init_state :: "nat \<Rightarrow> (bool \<times> (nat \<Rightarrow> na
 
 
       thm Pre_BFS_Impl.pre_bfs2_def 
-lemma PP: "Pre_BFS_Impl set_pick_time" by(simp add: Pre_BFS_Impl_def)
+lemma PP: "\<And>c. Pre_BFS_Impl (set_pick_time c)" by(simp add: Pre_BFS_Impl_def)
 
 
 lemma (in -) hn_refine_Some[sepref_fr_rules]: " hn_refine (hn_val Id s' s)
@@ -148,29 +167,31 @@ declare rbt_delete_time_logN_mono [intro]
         itypeI[Pure.of t "TYPE(nat)"]
         itypeI[Pure.of c "TYPE('ig)"]  
         \<comment> \<open>Declare parameters to operation identification\<close>
+      assumes inbounds: "s < N" and
+         inboundsAll: "\<forall>x\<in>Graph.V (absG c). x < N" 
       shows
-
+  
   "hn_refine (
         hn_ctxt (isG) c ci 
       * hn_val nat_rel s si 
       * hn_val nat_rel t ti) (?c::?'c Heap) ?\<Gamma>' ?R (PR_CONST op_bfs c s t)"
       unfolding op_bfs_def PR_CONST_def      
       apply(subst Augmenting_Path_BFS.bfs2_def) apply(simp add: Augmenting_Path_BFS_def)
-      unfolding Pre_BFS_Impl.pre_bfs2_def[OF PP]
-      unfolding Pre_BFS_Impl.inner_loop_def[OF PP]  unfolding  extract_rpath_def nfoldliIE_def nfoldli_def 
-      using [[id_debug, goals_limit = 2]]
-      unfolding monadic_WHILE_aux Pre_BFS_Impl.loopguard_def[OF PP] 
+      unfolding Pre_BFS_Impl.pre_bfs2_def[OF PP[of "(card (Graph.V (absG c)))"]]  
+      unfolding Pre_BFS_Impl.inner_loop_def[OF PP[of "(card (Graph.V (absG c)))"]]  unfolding  extract_rpath_def nfoldliIE_def nfoldli_def 
+      using [[id_debug, goals_limit = 3]]
+      unfolding monadic_WHILE_aux unfolding Pre_BFS_Impl.loopguard_def[OF PP[of "(card (Graph.V (absG c)))"]] 
       unfolding set_pick_time_def set_isempty_time_def set_delete_time_def map_dom_member_time_def
           map_update_time_def set_insert_time_def set_empty_time_def map_lookup_time_def list_append_time_def
-
+      using inbounds  inboundsAll 
   apply sepref_dbg_preproc
   apply sepref_dbg_cons_init
   apply sepref_dbg_id 
      apply sepref_dbg_monadify
 
      apply sepref_dbg_opt_init
-                                        
-  apply sepref_dbg_trans_keep 
+                                       
+  apply sepref_dbg_trans_keep                
 
   apply sepref_dbg_opt
   apply sepref_dbg_cons_solve \<comment> \<open>Frame rule, recovering the invalidated list 
@@ -182,8 +203,9 @@ declare rbt_delete_time_logN_mono [intro]
     concrete_definition (in -) bfs_impl uses Impl_Succ.bfs_impl
       \<comment> \<open>Extract generated implementation into constant\<close>
     prepare_code_thms (in -) bfs_impl_def
-   
-    lemmas bfs_impl_fr_rule = bfs_impl.refine[OF this_loc,to_hfref]  
+
+     
+  lemmas bfs_impl_fr_rule = bfs_impl.refine[OF this_loc, to_hfref]
   
   end
 
