Examples/EdmondsKarp_Maxflow/EdmondsKarp_Time.thy
@@ -3,6 +3,9 @@ theory EdmondsKarp_Time
  (*    "SepLogicTime_RBTreeBasic.Asymptotics_2D" 
       \<longrightarrow> Cannot join unrelated theory certificates SepLogicTime_RBTreeBasic.Asymptotics_2D:321 and SepLogicTime_RBTreeBasic.RBTree_Impl:4570
   *)
+
+  
+    "../../Refine_Imperative_HOL/IICF/Impl/IICF_RbtMap_Map"
 begin
  
 lemma "(\<lambda>x::nat. real ((3 ))) \<in> \<Theta>(\<lambda>(x). real 1)" 
@@ -14,8 +17,17 @@ lemma "(\<lambda>x. real ((32 ))) \<in> \<Theta>\<^sub>2(\<lambda>(V::nat,E::nat
 lemma "(\<lambda>x. real ((rbt_insert_logN 1 ))) \<in> \<Theta>\<^sub>2(\<lambda>(V::nat,E::nat). 1)" 
   apply (subst surjective_pairing) by auto2
 
-lemma "edka_cost \<in> \<Theta>\<^sub>2(\<lambda>(V::nat,E::nat). V * E * E * ln V + V * E * V * ln V)"
+lemma edka_runt: "edka_cost \<in> \<Theta>\<^sub>2(\<lambda>(V::nat,E::nat). (real V * E) * V + (V * E) * E * ln V )"
   apply (subst surjective_pairing)
   unfolding edka_cost_simp by auto2
+
+
+lemma final_running_time: "edka_cost \<in> \<Theta>\<^sub>2(\<lambda>(V::nat,E::nat). (V * E) * (V + E * ln V) )"
+proof -
+  have *:  "\<And>E V::nat. (V * E) * (V + E * ln V) = (real V * E) * V + (V * E) * E * ln V "  
+    by (simp add: distrib_left)  
+  show ?thesis unfolding * using edka_runt  
+    by simp
+qed 
 
 end
