Examples/EdmondsKarp_Maxflow/Graph_Impl.thy
@@ -15,17 +15,19 @@ locale Impl_Succ =
   fixes ifT :: "'ig itself"
   fixes succ :: "'ga \<Rightarrow> node \<Rightarrow> node list nrest"
   fixes isG :: "'ga \<Rightarrow> 'gi \<Rightarrow> assn"
-  fixes succ_impl :: "'gi \<Rightarrow> node \<Rightarrow> node list Heap"
- 
+  fixes succ_impl :: "'gi \<Rightarrow> node \<Rightarrow> node list Heap" 
+  fixes N :: "node" 
 
   (*assumes [constraint_rules]: "precise isG"*)
   assumes si_rule[sepref_fr_rules]: "(uncurry succ_impl,(uncurry succ)) \<in> [\<lambda>(c,u). u\<in>Graph.V (absG c)]\<^sub>a isG\<^sup>k *\<^sub>a (pure nat_rel)\<^sup>k \<rightarrow> list_assn (pure nat_rel)"
-begin                
+
+begin
 term "Impl_Succ   "
-  lemma this_loc: "Impl_Succ absG succ isG succ_impl " apply unfold_locales (* apply simp apply simp 
+  lemma this_loc: "Impl_Succ absG succ isG succ_impl" apply unfold_locales (* apply simp apply simp 
     using si_rule . *) done
 
   sepref_register "succ" :: "'ig \<Rightarrow> node \<Rightarrow> node list nrest" (* TODO: Will not work if succ is not a constant! *) 
+  print_theorems
 end
 
 
