Refine_Imperative_HOL/IICF/Impl/IICF_ArrayMap_Map.thy
@@ -1,0 +1,184 @@
+theory IICF_ArrayMap_Map
+  imports "../Intf/IICF_Map" "SepLogicTime_RBTreeBasic.RBTree_Impl"
+begin
+
+(* inspired by Separation_Logic_Imperative_HOL/Examples/Array_Map_Impl *)
+
+  subsection "Array Map"
+
+  type_synonym 'v array_map = "'v option array"
+
+  definition "iam_of_list l \<equiv> (\<lambda>i. if i<length l then l!i else None)"
+
+  lemma finite_dom_iam_of_list: "finite (dom (iam_of_list l))"
+    by(auto intro: subset_eq_atLeast0_lessThan_finite
+          simp: iam_of_list_def domIff split: if_splits)
+
+
+  definition is_liam   where
+    "is_liam s m a \<equiv> \<exists>\<^sub>Al f. snd a\<mapsto>\<^sub>rf * fst a\<mapsto>\<^sub>al * \<up>(length l=s \<and> card (dom m) = f \<and> m=iam_of_list l)"
+
+
+  definition new_liam :: "nat \<Rightarrow> (('a::{heap}) array_map \<times> 'b::{heap,zero} ref) Heap"  where
+    "new_liam n = do { a \<leftarrow> Array.new n None; s\<leftarrow>Ref.ref 0; return (a,s) } "
+
+lemma return_rule':
+  "<$1> return x <\<lambda>r. \<up>(r = x)>" by auto2
+
+
+schematic_goal "\<And>x xa. x \<mapsto>\<^sub>a replicate n None * xa \<mapsto>\<^sub>r 0 * $0\<Longrightarrow>\<^sub>A xa \<mapsto>\<^sub>r 0 * x \<mapsto>\<^sub>a ?f51 x xa  * $0"
+  apply solve_entails oops
+ 
+lemma new_liam_rule: "<$(n+3)> new_liam n <is_liam n (Map.empty)>" unfolding new_liam_def is_liam_def
+    apply(sep_auto heap: ref_rule return_rule' )
+    prefer 3 unfolding zero_time apply solve_entails by (auto simp: iam_of_list_def) 
+
+lemma mop_map_empty_rule:
+  "s+3\<le>t \<Longrightarrow> hn_refine (emp) (new_liam s) emp (is_liam s) (PR_CONST (mop_map_empty t))"
+  unfolding autoref_tag_defs mop_map_empty_def  
+  apply (rule extract_cost_otherway[OF _ new_liam_rule, where Cost_lb="s+3" and F=emp])
+    apply solve_entails+
+  by auto 
+
+thm mop_map_empty_rule[to_hfref]
+
+definition "mop_map_empty_fs s t = SPECT [ Map.empty \<mapsto> t]"
+
+context
+  fixes s::nat and t ::  " nat"
+begin
+  sepref_register "  (mop_map_empty_fs s t )" 
+  print_theorems 
+end
+
+  lemma  mop_map_empty_fs: "tt \<le> TTT Q (SPECT [ Map.empty \<mapsto> t  ]) 
+        \<Longrightarrow> tt \<le> TTT Q (mop_map_empty_fs s t )" unfolding mop_map_empty_fs_def by simp
+
+
+  definition "mop_map_empty_fixed_length s = mop_map_empty "
+  context fixes s :: nat begin
+      sepref_register " (mop_map_empty_fixed_length s)"
+  print_theorems 
+
+  (*    lemma [def_pat_rules]: "mop_map_empty_fixed_length$s \<equiv> UNPROTECT (mop_map_empty_fixed_length s)"
+      by simp *)
+  end
+
+lemma mop_map_empty_add_mn: "mop_map_empty = mop_map_empty_fs s"  by(auto simp: mop_map_empty_def mop_map_empty_fs_def)
+
+lemma mop_map_empty_rule'[sepref_fr_rules]:
+  "s+3\<le>n \<Longrightarrow> hn_refine (emp) (new_liam s) emp (is_liam s) (PR_CONST (mop_map_empty_fs s n))"
+  unfolding mop_map_empty_fs_def apply(rule mop_map_empty_rule[unfolded mop_map_empty_def]) by simp
+
+term RECT
+thm sep_heap_rules
+thm sep_decon_rules
+
+definition update_liam where
+    "update_liam m k v = do {
+          ov \<leftarrow> Array.nth (fst m) k;
+          a \<leftarrow> Array.upd k (Some v) (fst m);
+          (if ov = None then do {
+              s \<leftarrow> Ref.lookup (snd m);
+              Ref.update (snd m) (s+1);
+              return (a,snd m)
+            } else return (a, snd m))
+        }
+      "
+
+
+ 
+
+thm return_rule
+thm return_rule
+lemma zz: "xs!i = n \<Longrightarrow> xs[i:=n] = xs" by auto
+
+lemma "<$2> if c=0 then return d else return 0 <\<lambda>r. \<up>(r = 0)>\<^sub>t"
+  apply(sep_auto) oops
+
+lemma knotin_dom_iam_of_listI: "l ! k = None \<Longrightarrow> k \<notin> dom (iam_of_list l)"
+  by(auto simp: iam_of_list_def split: if_splits)
+
+lemma kin_dom_iam_of_listI: "k < length l \<Longrightarrow> l ! k = Some y \<Longrightarrow>  k \<in> dom (iam_of_list l) "
+  by(auto simp: iam_of_list_def)
+
+lemma iam_of_list_update: "k < length l \<Longrightarrow> iam_of_list (l[k := Some v]) = iam_of_list l(k \<mapsto> v)"   
+  by (auto simp: iam_of_list_def split: if_splits)
+ 
+
+lemma update_liam_rule: "k<n \<Longrightarrow> <is_liam n M m * $6> update_liam m k v <\<lambda>r. is_liam n (M(k:=Some v)) r >\<^sub>t"
+  unfolding update_liam_def is_liam_def
+  apply(sep_auto heap: nth_rule lookup_rule update_rule return_rule')
+    apply(auto simp:   zz  card_insert finite_dom_iam_of_list
+              set_minus_singleton_eq knotin_dom_iam_of_listI iam_of_list_update )
+  apply(sep_auto heap: return_rule')    
+   apply(auto intro!: card_Suc_Diff1   simp:    iam_of_list_update finite_dom_iam_of_list )
+  by(auto simp: iam_of_list_def) 
+
+
+lemma mop_set_insert_rule[sepref_fr_rules]:
+  "(uncurry2 update_liam, uncurry2 (PR_CONST (mop_map_update t)))
+     \<in> [\<lambda>((a, b), x). 6 \<le> t a \<and> b < mn]\<^sub>a (is_liam mn)\<^sup>d *\<^sub>a nat_assn\<^sup>k *\<^sub>a id_assn\<^sup>k \<rightarrow> is_liam mn"
+  apply sepref_to_hoare 
+  unfolding mop_map_update_def autoref_tag_defs
+  apply (rule extract_cost_otherway'[OF _  update_liam_rule ])
+  by (auto simp: emb'_def | solve_entails; auto)+  
+
+
+definition dom_member_liam where
+    "dom_member_liam m k = do { f \<leftarrow> Array.nth (fst m) k; return (f \<noteq> None) }"
+
+
+lemma dom_member_liam_rule: "k<n  \<Longrightarrow> <is_liam n M m * $2> dom_member_liam m k <\<lambda>r. is_liam n M m * \<up>(r\<longleftrightarrow>k\<in>dom M)  >\<^sub>t"
+  unfolding dom_member_liam_def is_liam_def
+  apply(sep_auto heap: nth_rule return_rule' )
+  by(auto simp: iam_of_list_def)
+
+
+lemma mop_mem_set_rule[sepref_fr_rules]:
+  "2 \<le> t M \<Longrightarrow> x < n \<Longrightarrow>
+    hn_refine (hn_val Id x x' * hn_ctxt (is_liam n) M p)
+     (dom_member_liam p x')
+     (hn_ctxt (pure Id) x x' * hn_ctxt (is_liam n) M p) id_assn ( PR_CONST (mop_map_dom_member t) $ M $ x)"
+  apply sepref_to_hoare 
+  unfolding autoref_tag_defs mop_map_dom_member_def
+  apply (rule extract_cost_otherway'[OF _  dom_member_liam_rule])  
+  by (auto simp: emb'_def | solve_entails; auto)+   
+
+
+
+
+
+
+
+definition nth_liam where
+    "nth_liam m k = do { f \<leftarrow> Array.nth (fst m) k; return (the f) }"
+
+lemma nth_liam_rule: "k<n \<Longrightarrow> k \<in> dom M \<Longrightarrow> <is_liam n M m * $2> nth_liam m k <\<lambda>r. is_liam n M m * \<up>(r=the (M k))>\<^sub>t"
+  unfolding nth_liam_def is_liam_def
+  apply(sep_auto heap: nth_rule return_rule' )
+  by(auto simp: iam_of_list_def)
+
+
+
+
+
+lemma mop_map_lookup_rule[sepref_fr_rules]:
+  "2 \<le> t M \<Longrightarrow> x < n \<Longrightarrow> 
+    hn_refine (hn_val Id x x' * hn_ctxt (is_liam n) M p)
+     (nth_liam p x')
+     (hn_ctxt (pure Id) x x' * hn_ctxt (is_liam n) M p) id_assn ( PR_CONST (mop_map_lookup t) $ M $ x)"
+  apply sepref_to_hoare
+  unfolding autoref_tag_defs mop_map_lookup_def 
+  apply(rule hnr_ASSERT) 
+  apply (rule extract_cost_otherway'[OF _ nth_liam_rule] )
+    by (auto | solve_entails; auto)+  
+
+
+
+
+
+
+
+
+end
